examples/guess: guess_state with contract

examples/guess.v
@@ -1,5 +1,5 @@
 From Coq Require Import Arith String Streams.
-From FreeSpec.Core Require Import Core.
+From FreeSpec.Core Require Import Core CoreFacts.
 
 Open Scope nat_scope.
 
@@ -17,7 +17,7 @@ Definition read_nat `{Provide ix CONSOLE} (u : unit) : impure ix nat :=
 Definition write `{Provide ix CONSOLE} (s : string) : impure ix unit :=
   request (Write s).
 
-(* definition of a semantic for the [CONSOLE] interface *)
+(** * Definition of a semantic for the [CONSOLE] interface *)
 CoFixpoint console (in_flow : Stream nat) (out_flow : list string): semantics (CONSOLE) :=
   mk_semantics (fun α (e : CONSOLE α) =>
                   match e with
@@ -25,7 +25,7 @@ CoFixpoint console (in_flow : Stream nat) (out_flow : list string): semantics (C
                   | Write s => (tt, console in_flow (s :: out_flow))
                   end).
 
-(* the guess game loop logic *)                  
+(** * The guess game loop logic *)                  
 Fixpoint guess `{Provide ix CONSOLE} (target max_attempt : nat)
   : impure ix unit :=
   match max_attempt with 
@@ -43,12 +43,84 @@ Fixpoint guess `{Provide ix CONSOLE} (target max_attempt : nat)
         guess target m
   end.
 
-(* aux functions to generate infinite flows *)
+Inductive game_state : Type :=
+| Won : game_state
+| GameOver : game_state
+| GSmall : game_state
+| GBig : game_state
+| GEqual : game_state.
+
+Record game : Type := mkGame
+  { target : nat
+  ; max_attempt : nat 
+  ; state : game_state
+  }.
+
+(** Simplified witness states *)
+Inductive guess_state : Type :=
+| Retry : guess_state 
+| Guessed : guess_state.
+
+Definition guess_update (target : nat)
+  (g : guess_state) (α: Type) (c : CONSOLE α) (x : α) : guess_state :=
+  match g,c,x with 
+  | Retry, ReadNat _, n =>
+    if n =? target then Guessed else Retry 
+  | _, _, _ => g end.
+
+Inductive guess_caller_obligation : guess_state -> forall (α : Type),
+  CONSOLE α -> Prop :=
+  (* can always retry for now *)
+  | retry (u : unit) (g : guess_state)
+   : guess_caller_obligation g nat (ReadNat u)
+  
+  (* write 'Won !' iff the target is guessed *)
+  | write_msg (msg : string) (g : guess_state)
+              (H : g = Guessed <-> msg = "Won !")
+    : guess_caller_obligation g unit (Write msg).
+
+Inductive no_callee_obligation (g : guess_state) (α : Type)
+  (c : CONSOLE α) (x : α) : Prop :=
+  | mk_no_callee_obligation : no_callee_obligation g α c x.
+
+Definition guess_contract (target : nat) : contract CONSOLE guess_state :=
+  {| witness_update := guess_update target
+   ; caller_obligation := guess_caller_obligation
+   ; callee_obligation := no_callee_obligation
+  |}.
+
+(* always allow retry (read_nat) *)
+Lemma allow_retry `{Provide ix CONSOLE} (g : guess_state) (u : unit)
+  : forall t : nat, pre (to_hoare (guess_contract t) (read_nat u)) g.
+Proof.
+  intro t.
+  prove impure.
+  constructor.
+Qed.
+
+Definition guess10 `{Provide ix CONSOLE} (target : nat)
+  : impure ix unit :=
+  guess target 10.
+
+Lemma write_won_if_guessed `{Provide ix CONSOLE} (g : guess_state) (u : unit)
+  : forall t : nat, pre (to_hoare (guess_contract t) (guess10 t)) g.
+Admitted.
+
+(** * Aux functions to generate infinite flows *)
 CoFixpoint rep_inf {A : Type} (n:A) : Stream A := 
   Cons n (rep_inf n).
 
 CoFixpoint nat_inf (n:nat) : Stream nat := 
   Cons n (nat_inf (S n)).
+
+(** * Execution examples *)
+Definition base_semantic := console (nat_inf 0) [].
+
+Compute (eval_effect base_semantic (ReadNat _)).
+(* >> 0 *)
+
+Compute (exec_effect base_semantic (Write "hello world !")).
+(* >> _ ["hello world !"] *)
 
 Compute (exec_impure (console (rep_inf 10) []) (guess 10 20)).
 (* >> out_flow: ["Won !"; "Guess the number:"] *)
